new file (HahnOmega) + more lemmas about traces

HahnTrace.v
@@ -2,31 +2,207 @@
 (** * Lemmas about traces (finite or infinite sequences) *)
 (******************************************************************************)
 
-Require Import HahnBase HahnList.
-Require Import Omega.
+Require Import HahnBase HahnList HahnSets HahnOmega.
+Require Import Omega IndefiniteDescription.
 
 Set Implicit Arguments.
 
+Lemma set_infinite_natE (s : nat -> Prop) (INF: ~ set_finite s) n :
+  exists m, s m /\ length (filterP s (seq 0 m)) = n.
+Proof.
+  assert (IMP: forall findom, exists x, s x /\ ~ In x findom).
+  { unfold set_finite in *; apply NNPP; intro X; clarify_not.
+    eapply INF; eexists; ins; apply NNPP; intro Y; eauto. }
+  apply functional_choice in IMP; destruct IMP as [nin IMP].
+  assert (exists m, s m /\ n <= length (filterP s (seq 0 m))).
+  { induction n; desf.
+    1: exists (nin nil); split; [apply IMP | omega].
+    exists (nin (seq 0 (S m))); split; [apply IMP|].
+    rewrite seq_split0 with (a := m).
+    rewrite filterP_app, length_app; ins; desf; ins; omega.
+    specialize (IMP (seq 0 (S m))); desf.
+    rewrite in_seq0_iff in IMP0; omega. }
+  desf; rewrite Nat.le_lteq in *; desf; eauto.
+  clear - H0; induction m; ins.
+  replace (seq 0 0) with (@nil nat) in H0; ins; omega.
+  replace (S m) with (m + 1) in H0; try omega.
+  rewrite seq_add, filterP_app, length_app in H0; ins.
+  replace (seq m 1) with (m :: nil) in H0; ins; desf; ins.
+  1: rewrite Nat.add_1_r, Nat.lt_succ_r, Nat.le_lteq in *; desf; eauto.
+  rewrite Nat.add_0_r in *; eauto.
+Qed.
+
+(** Prepend a finite list to an infinite sequence *)
+
+Definition trace_prepend A (l : list A) (fl : nat -> A) n :=
+  if Nat.ltb n (length l) then nth n l (fl 0)
+  else fl (n - length l).
+
+
+(******************************************************************************)
+(** Lemmas about [trace_prepend] *)
+(******************************************************************************)
+
+Lemma trace_prepend_fst A (l: list A) fl n (LT : n < length l) :
+  trace_prepend l fl n = nth n l (fl 0).
+Proof.
+  unfold trace_prepend; desf; f_equal; omega.
+Qed.
+
+Lemma trace_prepend_fst0 A (l: list A) fl x :
+  trace_prepend (x :: l) fl 0 = x.
+Proof.
+  ins.
+Qed.
+
+Lemma trace_prepend_snd A (l: list A) fl n :
+  trace_prepend l fl (length l + n) = fl n.
+Proof.
+  unfold trace_prepend; desf; f_equal; omega.
+Qed.
+
+Lemma trace_prepend_snd0 A (l: list A) fl :
+  trace_prepend l fl (length l) = fl 0.
+Proof.
+  unfold trace_prepend; desf; f_equal; omega.
+Qed.
+
+Lemma trace_prepend_app A (l l' : list A) fl :
+  trace_prepend (l ++ l') fl = trace_prepend l (trace_prepend l' fl).
+Proof.
+  unfold trace_prepend; extensionality n.
+  rewrite length_app, nth_app; desf; try omega.
+  all: first [apply nth_indep | f_equal]; omega.
+Qed.
+
+Hint Rewrite
+     filterP_app
+     length_app
+     trace_prepend_fst0
+     trace_prepend_snd
+     trace_prepend_snd0
+     trace_prepend_app : trace_prepends.
+
+Lemma map_trace_prepend_geq A (l: list A) fl n (LT: length l <= n) :
+  map (trace_prepend l fl) (seq 0 n) =
+    l ++ map fl (seq 0 (n - length l)).
+Proof.
+  unfold trace_prepend.
+  rewrite seq_split with (x := length l); ins.
+  rewrite map_app.
+  rewrite map_nth_seq with (d := fl 0); [|by ins; desf].
+  rewrite map_seq_shift with (g := fl) (b := 0); ins.
+  desf; try f_equal; omega.
+Qed.
+
+Lemma map_trace_prepend_lt A (l: list A) fl n (LT: n < length l) :
+  exists l' a l'',
+    l = l' ++ a :: l'' /\ length l' = n /\
+    map (trace_prepend l fl) (seq 0 n) = l'.
+Proof.
+  unfold trace_prepend.
+  destruct (Nat.le_exists_sub n (length l)) as (p & X & _);
+    try omega.
+      rewrite Nat.add_comm in X.
+  apply length_eq_add in X; desf.
+  rewrite length_app in *; destruct l''; ins; try omega.
+  repeat eexists.
+  eapply map_nth_seq with (d := fl 0); ins; desf; try omega.
+  rewrite nth_app; desf; try omega.
+Qed.
+
+
+Lemma set_finite_prepend A (l : list A) (fl : nat -> A) (f : A -> Prop) :
+  set_finite (set_map (trace_prepend l fl) f) <-> set_finite (set_map fl f).
+Proof.
+  unfold trace_prepend, set_finite, set_map.
+  split; ins; desf.
+  { exists (map (fun x => x - length l) findom); intro y; ins.
+    rewrite in_map_iff.
+    specialize (H (y + length l)); desf; eauto; try omega.
+    exists (y + length l); rewrite Nat.add_sub in *; eauto. }
+  { exists (seq 0 (length l) ++ map (fun x => x + length l) findom);
+    intro y; ins.
+    rewrite in_app_iff, in_seq0_iff, in_map_iff; desf; eauto.
+    apply H in IN.
+    right; eexists; split; eauto; omega.
+  }
+Qed.
+
+(******************************************************************************)
 (** Finite or infinite traces of [A] elements. *)
+(******************************************************************************)
 
 Inductive trace (A : Type) : Type :=
 | trace_fin (l : list A)
 | trace_inf (fl : nat -> A).
 
-Definition trace_seq A (t t' : trace A) :=
+(** [trace_app] concatenates two traces *)
+
+Definition trace_app A (t t' : trace A) :=
   match t, t' with
   | trace_fin l, trace_fin l' => trace_fin (l ++ l')
   | trace_fin l, trace_inf f =>
-    trace_inf (fun n => if Nat.ltb n (length l) then nth n l (f 0)
-                        else f (n - length l))
+    trace_inf (trace_prepend l f)
   | trace_inf f, _ => trace_inf f
   end.
+
+(** [trace_map f t] applies [f] to all the elements of [t] *)
 
 Definition trace_map A B (f : A -> B) (t : trace A) : trace B :=
   match t with
   | trace_fin l => trace_fin (map f l)
   | trace_inf fl => trace_inf (fun x => f (fl x))
   end.
+
+(** Returns the length of a trace *)
+
+Definition trace_length A (t : trace A) : nat_omega :=
+  match t with
+  | trace_fin l => NOnum (length l)
+  | trace_inf fl => NOinfinity
+  end.
+
+(** [trace_in a t] returns true iff [a] is an element of the trace [t] *)
+
+Definition trace_in A (a : A) (t : trace A) :=
+  match t with
+  | trace_fin l => In a l
+  | trace_inf fl => exists n, a = fl n
+  end.
+
+(** [trace_nth n t d] returns the [n]th element of trace [t]
+   or the default element [d], if [n] exceeds the trace's length. *)
+
+Definition trace_nth (n : nat) A (t : trace A) (d : A) : A :=
+  match t with
+  | trace_fin l => nth n l d
+  | trace_inf fl => fl n
+  end.
+
+(** [trace_filter f t] returns the sub-trace of [t] whose elements
+satisfy the predicate [f]. *)
+
+Definition trace_filter A (f : A -> Prop) (t : trace A) : trace A :=
+  match t with
+  | trace_fin l => trace_fin (filterP f l)
+  | trace_inf fl =>
+    let s := excluded_middle_informative (set_finite (set_map fl f)) in
+    match s with
+    | left FIN =>
+        let B := set_finite_nat_bounded FIN in
+        let n := proj1_sig (constructive_indefinite_description _ B) in
+        trace_fin (filterP f (map fl (seq 0 (S n))))
+    | right INF =>
+        trace_inf
+          (fun n =>
+           let H := set_infinite_natE INF n in
+           let H0 := constructive_indefinite_description _ H in
+           fl (proj1_sig H0))
+    end
+  end.
+
+(** Is a trace a prefix of another trace? *)
 
 Definition trace_prefix A (t t' : trace A) :=
   match t, t' with
@@ -36,33 +212,181 @@ Definition trace_prefix A (t t' : trace A) :=
   | trace_inf f, trace_inf f' => forall x, f x = f' x
   end.
 
-Lemma trace_prefix_seq A (t t' : trace A) :
-  trace_prefix t (trace_seq t t').
+(******************************************************************************)
+(** Basic lemmas *)
+(******************************************************************************)
+
+Lemma trace_nth_indep (n : nat) A (t : trace A)
+      (LT : NOmega.lt_nat_l n (trace_length t)) (d d' : A) :
+  trace_nth n t d = trace_nth n t d'.
 Proof.
-  destruct t, t'; ins; desf; eauto using nth_indep; done.
+  destruct t; ins; desf; auto using nth_indep.
+Qed.
+
+Lemma trace_length_app A (t t' : trace A) :
+  trace_length (trace_app t t') =
+  NOmega.add (trace_length t) (trace_length t').
+Proof.
+  destruct t, t'; ins; auto using length_app.
+Qed.
+
+Lemma trace_in_app A (a : A) (t t' : trace A) :
+  trace_in a (trace_app t t') <->
+  trace_in a t \/ trace_length t <> NOinfinity /\ trace_in a t'.
+Proof.
+  split; destruct t, t'; ins; unfold trace_prepend in *;
+    desf; rewrite ?in_app_iff in *; desf;
+    eauto using nth_In; vauto.
+  all: try solve [right; split; ins; eauto].
+  apply In_nth with (d := fl 0) in H; desf; exists n; desf; ins.
+  exists (n + length l); desf; try f_equal; omega.
+Qed.
+
+Lemma trace_nth_app (n : nat) A (t t' : trace A) (d : A) :
+  trace_nth n (trace_app t t') d =
+  ifP NOmega.lt_nat_l n (trace_length t) then trace_nth n t d
+  else trace_nth (NOmega.sub_nat_l n (trace_length t)) t' d.
+Proof.
+  destruct t, t'; ins; unfold trace_prepend in *;
+    desf; try rewrite app_nth; desf;
+      auto using nth_indep; omega.
+Qed.
+
+Lemma trace_in_map A (a : A) B (f : B -> A) (t : trace B) :
+  trace_in a (trace_map f t) <-> exists x, trace_in x t /\ f x = a.
+Proof.
+  destruct t; ins; try rewrite in_map_iff; split; ins; desf; eauto.
+Qed.
+
+Lemma trace_nth_map (n : nat) A (a : A) B (f : B -> A) (t : trace B) d :
+  trace_nth n (trace_map f t) (f d) = f (trace_nth n t d).
+Proof.
+  destruct t; ins; apply map_nth.
+Qed.
+
+Lemma trace_in_filter A (a : A) (f : A -> Prop) (t : trace A) :
+  trace_in a (trace_filter f t) <-> trace_in a t /\ f a.
+Proof.
+  destruct t; ins; desf; ins; rewrite ?in_filterP_iff, ?in_map_iff; ins.
+  all: split; ins; desf; splits; eauto.
+  all: try (eexists; try split; ins).
+  all: destruct (constructive_indefinite_description); ins; desf.
+  { in_simp; apply l in H0; omega. }
+  revert a0.
+  instantiate (1 := length (filterP (fl ↓₁ f) (seq 0 n0))).
+  destruct (lt_eq_lt_dec x n0) as [[LT|]|LT]; desf.
+  unfold set_map.
+  all: rewrite (seq_split0 LT), filterP_app, length_app;
+    ins; desf; ins; omega.
+Qed.
+
+
+Lemma trace_filter_app A (f : A -> Prop) (t t' : trace A)
+      (IMP: trace_length (trace_filter f t) <> NOinfinity ->
+            trace_length t <> NOinfinity) :
+  trace_filter f (trace_app t t') =
+  trace_app (trace_filter f t)
+            (trace_filter f t').
+Proof.
+  destruct t; ins; desf; ins; desf.
+  all: try solve [destruct IMP; ins]; clear IMP.
+  all: repeat destruct (constructive_indefinite_description); ins; desf.
+  all: try solve [exfalso; rewrite set_finite_prepend in *; ins].
+    by rewrite filterP_app in *.
+  { unfold set_map in *.
+    destruct (le_lt_dec (length l) (S x)).
+    - rewrite map_trace_prepend_geq; ins.
+      unfold trace_prepend in *.
+      rewrite filterP_app.
+      do 2 f_equal.
+      eapply filterP_map_seq_eq; simpl; eauto.
+      ins; forward apply (l0 (length l + i)); desf; try omega.
+        by rewrite minus_plus.
+      ins; eapply l1 in H; omega.
+    - eapply map_trace_prepend_lt with (fl := fl) in l2; desf.
+      rewrite l4, filterP_app, appA; clear l4.
+      f_equal.
+      symmetry; rewrite app_eq_prefix, app_eq_nil, ?filterP_eq_nil.
+      remember (a :: l'') as l; clear a l'' Heql.
+      split; ins.
+      apply in_split in IN; desf.
+        forward apply (l0 (length l' + length l2)); try omega.
+        by autorewrite with trace_prepends.
+      in_simp.
+      forward apply (l0 (length l' + (length l + x2))); try omega.
+      by autorewrite with trace_prepends.
+  }
+  { f_equal; extensionality y; ins.
+    destruct (constructive_indefinite_description); ins; desf.
+    erewrite <- length_map, <- filterP_map.
+    destruct (le_lt_dec (length l) x) as [LE|LT].
+    { rewrite map_trace_prepend_geq; ins.
+      autorewrite with trace_prepends.
+      rewrite filterP_map, length_map.
+      destruct (constructive_indefinite_description); ins; desf.
+      unfold set_map, trace_prepend in *; desf; try omega.
+      destruct (lt_eq_lt_dec (x - length l) x0) as [[LT|]|LT]; desf;
+      apply seq_split0 in LT; rewrite LT in *;
+        exfalso; revert a1; rewrite ?map_app, ?filterP_app, ?length_app;
+          ins; desf; ins; omega. }
+    eapply map_trace_prepend_lt with (fl := fl) in LT; desf.
+    rewrite filterP_app, LT1; red in a.
+    autorewrite with trace_prepends in *; ins; desf.
+  }
+Qed.
+
+
+Lemma trace_prefix_app A (t t' : trace A) :
+  trace_prefix t (trace_app t t').
+Proof.
+  destruct t, t'; ins; unfold trace_prepend;
+    desf; eauto using nth_indep; done.
 Qed.
 
 Lemma trace_prefixE A (t t' : trace A) :
-  trace_prefix t t' <-> exists t'', t' = trace_seq t t''.
+  trace_prefix t t' <-> exists t'', t' = trace_app t t''.
 Proof.
-  split; ins; desf; eauto using trace_prefix_seq.
+  split; ins; desf; eauto using trace_prefix_app.
   destruct t, t'; ins; desf; desf.
   - by eexists (trace_fin _).
   - exists (trace_inf (fun x => fl (x + length l))).
-    f_equal; extensionality y; desf; eauto.
+    unfold trace_prepend; f_equal; extensionality y; desf; eauto.
     f_equal; omega.
   - exists (trace_fin nil); f_equal; extensionality x; eauto.
 Qed.
 
-Lemma trace_seqA A (t t' t'' : trace A) :
-  trace_seq (trace_seq t t') t'' =
-  trace_seq t (trace_seq t' t'').
+
+Lemma trace_prefix_refl A (t : trace A) :
+  trace_prefix t t.
 Proof.
-  unfold trace_seq; ins; desf; try now rewrite appA.
+  destruct t; ins; eauto using app_nil_end.
+Qed.
+
+Lemma trace_prefix_trans A (t t' t'' : trace A) :
+  trace_prefix t t' ->
+  trace_prefix t' t'' ->
+  trace_prefix t t''.
+Proof.
+  destruct t, t', t''; ins; desf; try rewrite <- H0; eauto.
+    by rewrite appA; vauto.
+  forward apply H0 with (i := i) (d := d);
+    rewrite ?length_app, ?nth_app;
+    ins; desf; omega.
+Qed.
+
+
+Lemma trace_appA A (t t' t'' : trace A) :
+  trace_app (trace_app t t') t'' = trace_app t (trace_app t' t'').
+Proof.
+  unfold trace_app; ins; desf; try by rewrite appA.
   all: f_equal; extensionality x; desf.
-  all: rewrite length_app, ?nth_app in *; desf; try omega.
-  auto using nth_indep.
-  all: f_equal; omega.
+  by rewrite trace_prepend_app.
+Qed.
+
+Lemma trace_app_assoc A (t t' t'' : trace A) :
+  trace_app t (trace_app t' t'') = trace_app (trace_app t t') t''.
+Proof.
+  symmetry; apply trace_appA.
 Qed.
 
 
